src/Examples.v
@@ -1,8 +1,12 @@
 Require Import AssociativeCommutative.
 
-Require Import Quote.
+Set Implicit Arguments.
+
 Require Import Arith.
 Require Import Permutation.
+Require Import List.
+Import ListNotations.
+Open Scope list.
 
 Instance nat_plus_AC : AssociativeCommutative nat plus eq.
 Proof.
@@ -18,7 +22,7 @@ Instance list_AC A : AssociativeCommutative (list A) (app (A:=A)) (Permutation (
 Proof.
   constructor; hnf.
   - intros.
-    rewrite List.app_assoc; auto.
+    rewrite app_assoc; auto.
   - intros.
     apply Permutation_app_comm.
   - constructor; hnf; intros; eauto.
@@ -29,21 +33,34 @@ Proof.
     eapply Permutation_app; eauto.
 Qed.
 
-Fixpoint op_tree_nat (vm: varmap nat) (t:binop_tree nat) :=
-  match t with
-  | Leaf x => x
-  | Atom i => varmap_find default_val i vm
-  | Node l r => op_tree_nat vm l + op_tree_nat vm r
-  end.
-
 Theorem nat_rewrite : forall (x y z w: nat),
     x + y + x + z + y + w =
     x + x + y + z + y + w.
 Proof.
   intros.
-  (* quote can't handle this *)
-  Fail match goal with
-       | [ |- ?t = _ ] =>
-         quote op_tree_nat in t using (fun t' => idtac t)
-       end.
-Abort.
+  match goal with
+  | [ |- ?t = ?t' ] =>
+    quote t; requote t'
+  end.
+  ac_simplify.
+  reflexivity.
+Qed.
+
+Theorem list_rewrite : forall A (x y z w: list A),
+    Permutation (x ++ y ++ x ++ z ++ y ++ w)
+                (x ++ x ++ y ++ z ++ y ++ w).
+Proof.
+  intros.
+  match goal with
+  | [ |- Permutation ?t ?t' ] =>
+    quote t; requote t'
+  end.
+  ac_simplify.
+  match goal with
+  (* note that ac_simplify reduces to a left associative tree of operations,
+    whereas [++] is parsed as right associative. *)
+  | [ |- Permutation (((((x ++ x) ++ y) ++ y) ++ z) ++ w)
+                    (((((x ++ x) ++ y) ++ y) ++ z) ++ w) ] =>
+    reflexivity
+  end.
+Qed.
